theories/L6_PCPS/case_fold.v
@@ -6,18 +6,17 @@ Unset Strict Unquote Universe Mode.
 Inductive cfold_step : exp -> exp -> Prop :=
 | cfold_step0 : forall (C : frames_t exp_univ_exp exp_univ_exp) x c e ces,
   (exists D ys E, C = D >:: Econstr3 x c ys >++ E) /\ In (c, e) ces ->
-  When (fun (r : unit) (s : unit) => true) ->
   cfold_step (C ⟦ Ecase x ces ⟧) (C ⟦ Rec e ⟧).
 
-Definition R_C_ctors {A} (C : exp_c A exp_univ_exp) : Set := {
+Definition R_ctors {A} (C : exp_c A exp_univ_exp) : Set := {
   ρ : M.tree (ctor_tag * list var) |
   forall x c ys, M.get x ρ = Some (c, ys) -> exists D E, C = D >:: Econstr3 (mk_var x) c ys >++ E }.
 
-Instance Preserves_R_C_R_C_ctors : Preserves_R_C _ _ (@R_C_ctors).
+Instance Preserves_R_R_ctors : Preserves_R _ _ (@R_ctors).
 Proof.
   intros A B fs f [ρ Hρ]; destruct f;
   try lazymatch goal with
-  | |- R_C_ctors (fs >:: Econstr3 ?x' ?c' ?ys') => rename x' into x, c' into c, ys' into ys
+  | |- R_ctors (fs >:: Econstr3 ?x' ?c' ?ys') => rename x' into x, c' into c, ys' into ys
   | _ => let x := fresh "x" with c := fresh "c" with ys := fresh "ys" with Hget := fresh "Hget" in
     exists ρ; intros x c ys Hget; destruct (Hρ x c ys Hget) as [D [E Heq]];
     match goal with |- exists _ _, _ >:: ?f = _ => exists D, (E >:: f); now subst end
@@ -27,19 +26,6 @@ Proof.
   - inversion Hget; now exists fs, <[]>.
   - destruct (Hρ x' c' ys' Hget) as [D [E Heq]]; subst. now exists D, (E >:: Econstr3 (mk_var x) c ys).
 Defined.
-
-(* TODO: move to prototype.v and make uncurry_proto use this *)
-Ltac mk_easy_delay :=
-  try lazymatch goal with
-  | |- ConstrDelay _ -> _ =>
-    clear; simpl; intros; lazymatch goal with H : forall _, _ |- _ => eapply H; try reflexivity; eauto end
-  | |- EditDelay _ -> _ =>
-    clear; simpl; intros; lazymatch goal with H : forall _, _ |- _ => eapply H; try reflexivity; eauto end
-  end.
-
-(* TODO: move to proto_util.v *)
-Definition trivial_S {A} (C : exp_c A exp_univ_exp) (e : univD A) : Set := unit.
-Instance Preserves_S_trivial_S : Preserves_S _ _ (@trivial_S). Proof. do 2 constructor. Defined.
 
 Fixpoint find_case (c : ctor_tag) (ces : list (ctor_tag * exp)) : option exp :=
   match ces with
@@ -54,13 +40,19 @@ Proof.
   rewrite <- Pos.eqb_neq in Hneq; now rewrite Hneq.
 Qed.
 
-Definition rw_cfold : rewriter exp_univ_exp cfold_step unit unit
-  (@trivial_delay_t) (@R_C_ctors) (@trivial_R_e) (@trivial_S).
+Definition rw_cfold' : rewriter exp_univ_exp cfold_step
+  trivial_delay_t (@R_ctors) trivial_S.
 Proof.
-  mk_rw; mk_easy_delay; [|do 2 constructor].
-  intros _ _ _ R C [x] ces [ρ Hρ] _ _ success failure.
-  destruct (M.get x ρ) as [[c ys]|] eqn:Hget; [|exact failure].
-  destruct (find_case c ces) as [e|] eqn:Hfind; [|exact failure].
-  apply (success c e); [split; [|now apply find_case_refines_In]|reflexivity].
-  destruct (Hρ x c ys Hget) as [D [E Heq]]; repeat eexists; eassumption.
+  mk_rw; mk_easy_delay; [|constructor; [assumption|do 2 constructor]].
+  unfold trivial_delay_t, delayD, Delayed_trivial_delay_t in *.
+  intros _ R C [x] ces d [ρ Hρ] _ success failure.
+  destruct (M.get x ρ) as [[c ys]|] eqn:Hget; [|cond_failure].
+  destruct (find_case c ces) as [e|] eqn:Hfind_case; [|cond_failure].
+  cond_success; eapply (success (mk_var x) ces e tt c e); [|reflexivity..].
+  split; [|now apply find_case_refines_In]; destruct (Hρ x c ys Hget) as [? [? ?]]; eauto.
 Defined.
+
+Definition rw_cfold : rewriter exp_univ_exp cfold_step trivial_delay_t (@R_ctors) trivial_S :=
+  Eval unfold rw_cfold', Fuel_Fix, rw_chain, rw_base, rw_id in rw_cfold'.
+
+Recursive Extraction rw_cfold.
